Mae files compile in refinements folder

rupicola/refinements/QExp.fst
@@ -6,12 +6,14 @@ open FStar.Tactics.V2
 module M = FStar.Monotonic.Pure
 
 let (<=) #a (wp1 wp2:pure_wp a) = pure_stronger a wp1 wp2
-let ret (#a:Type u#a) x : pure_wp a = pure_return a x
+let ret (#a:Type u#a) x : pure_wp a =
+  FStar.Monotonic.Pure.as_pure_wp
+  (fun p -> p x)
 
-let refv_wp (#a:Type u#a) (ref1 ref2:a -> Type0) (wpV:pure_wp (x:a{ref1 x})) : pure_wp (x:a{ref2 x}) =
-  reveal_opaque (`%pure_wp_monotonic) (pure_wp_monotonic u#a);
+let refv_wp #a (ref1 ref2:a -> Type0) (wpV:pure_wp (x:a{ref1 x})) : pure_wp (x:a{ref2 x}) =
   pure_bind_wp (x:a{ref1 x}) (x:a{ref2 x}) wpV (fun r ->
-    (fun (p:pure_post (x:a{ref2 x})) -> ref2 r /\ p r))
+    FStar.Monotonic.Pure.as_pure_wp
+      (fun (p:pure_post (x:a{ref2 x})) -> ref2 r /\ p r))
 
 (** Typing environment **)
 type env = var -> option Type0
@@ -105,8 +107,8 @@ let wp_app #_ #a #b wpF wpX =
 
 unfold
 val helper_app: #g :env ->
-                #a :Type u#a ->
-                #b :Type u#b ->
+                #a :Type ->
+                #b :Type ->
                 #wpF : spec_env g (a -> b) ->
                 f :fs_oexp g (a -> b) wpF ->
                 #wpX : spec_env g a ->
@@ -132,7 +134,7 @@ let wp_if #_ #a wpC wpT wpE =
 
 unfold
 val helper_if : #g :env ->
-                #a :Type u#a ->
+                #a :Type ->
                 #wpC : spec_env g bool ->
                 c   : fs_oexp g bool wpC ->
                 #wpT : spec_env g a ->
@@ -140,48 +142,48 @@ val helper_if : #g :env ->
                 #wpE : spec_env g a ->
                 e   : fs_oexp g a wpE ->
                 fs_oexp g a (wp_if wpC wpT wpE)
-let helper_if c t e =
+let helper_if #_ #_ #wpC c #wpT t #wpE e =
   fun fsG ->
-    M.elim_pure_wp_monotonicity_forall u#0 ();
-    M.elim_pure_wp_monotonicity_forall u#a ();
+    M.elim_pure_wp_monotonicity (wpC fsG);
+    M.elim_pure_wp_monotonicity (wpT fsG);
+    M.elim_pure_wp_monotonicity (wpE fsG);
     if c fsG then t fsG else e fsG
 
 val wp_lambda : #g :env ->
-                #a :Type u#0 ->
-                #b :Type u#b ->
-                wpBody:spec_env (extend a g) b ->
+                #a :Type ->
+                #b :Type ->
+                wpCtx:spec_env (extend a g) b ->
+                body:fs_oexp (extend a g) b wpCtx ->
                 spec_env g (a -> b)
 
-let wp_lambda #g #a #b wpBody fsG : pure_wp (a -> b) =
-  reveal_opaque (`%pure_wp_monotonic) (pure_wp_monotonic u#b);
+let wp_lambda #g #a #b wpCtx body fsG : pure_wp (a -> b) = (** Cezar: this seems to be exactly what F* generates **)
+  M.as_pure_wp
   fun (p:pure_post (a -> b)) ->
-    forall (f:a -> b).
-      (forall (p':pure_post b) (fsG':fs_env (extend a g)).
-        fsG == fs_tail fsG' ==>  wpBody fsG' p' ==>  p' (f (fs_hd fsG'))
-      ) ==>  p f
+    (forall x. wpCtx (fs_stack fsG x) (fun _ -> True)) /\
+    pure_return _ (fun x -> body (fs_stack fsG x)) p
+//    p (fun x -> body (fs_stack fsG x))
 
 unfold
 val helper_lambda : #g :env ->
                 #a :Type ->
                 #b :Type ->
-                #wpBody:spec_env (extend a g) b ->
-                f :fs_oexp g (a -> b) (wp_lambda wpBody) ->
-                fs_oexp (extend a g) b wpBody
-let helper_lambda #g #a f =
-  fun fsG -> f (fs_tail #a fsG) (fs_hd fsG)
+                #wpCtx:spec_env (extend a g) b ->
+                body :fs_oexp (extend a g) b wpCtx ->
+                fs_oexp g (a -> b) (wp_lambda wpCtx body)
+let helper_lambda #g #a #b #wpCtx body fsG =
+  (fun x -> body (fs_stack fsG x))
 
-val wp_lambda0' :
+val wp_lambda' :
   #g :env ->
-  #a :Type u#0 ->
-  #b :Type u#b ->
+  #a :Type ->
+  #b :Type ->
   wpCtx : spec_env (extend a g) b ->
   wpFun : (a -> pure_wp b) ->
   fs_oexp (extend a g) b wpCtx ->
-  fsG:fs_env g ->
-  pure_wp' (x:a -> PURE b (wpFun x))
+  spec_env g (x:a -> PURE b (wpFun x))
 
-let wp_lambda0' #g #a #b wpCtx wpFun body fsG =
-  fun (p:pure_post (x:a -> PURE b (wpFun x))) ->
+let wp_lambda' #g #a #b wpCtx wpFun body fsG : pure_wp (x:a -> PURE b (wpFun x))  =
+  let w : pure_wp' _ = fun (p:pure_post (x:a -> PURE b (wpFun x))) ->
     (forall (x: a) (p: pure_post b).
       wpFun x p ==>
       (wpCtx (fs_stack fsG x) (fun _ -> True) /\ (** Cezar: this is the only extra thing compared to the VC created by F* **)
@@ -190,28 +192,25 @@ let wp_lambda0' #g #a #b wpCtx wpFun body fsG =
         pure_return _ res p))
     //) /\ pure_return _ (fun x -> body (fs_stack fsG x)) p // Cezar: this is not accepted?
     ) /\ p (fun x -> body (fs_stack fsG x))
-
-let lem_wp_lambda'_monotonic #g #a #b wpCtx wpFun body fsG : Lemma (pure_wp_monotonic0 (x:a -> PURE b (wpFun x)) (wp_lambda0' #g #a #b wpCtx wpFun body fsG)) =
-  admit ()
-
-val wp_lambda' :
-  #g :env ->
-  #a :Type u#0 ->
-  #b :Type u#b ->
-  wpCtx : spec_env (extend a g) b ->
-  wpFun : (a -> pure_wp b) ->
-  fs_oexp (extend a g) b wpCtx ->
-  fsG:fs_env g ->
-  pure_wp (x:a -> PURE b (wpFun x))
-let wp_lambda' #g (#a:Type u#0) (#b:Type u#b) wpCtx wpFun body fsG : pure_wp (x:a -> PURE b (wpFun x)) =
-  lem_wp_lambda'_monotonic wpCtx wpFun body fsG;
-  reveal_opaque (`%pure_wp_monotonic) (pure_wp_monotonic u#b);
-  admit ();
-  wp_lambda0' #g #a #b wpCtx wpFun body fsG
+  in
+  assume (M.is_monotonic w);
+  M.as_pure_wp w
 
 
-unfold
-val helper_lambda' :
+
+  // fun (p:pure_post (x:a -> PURE b (wpFun x))) ->
+  //   (forall x. (* wpFun x (fun _ -> True) ==> *) wpCtx (fs_stack fsG x) (fun _ -> True)) /\
+  //   forall (f:(x:a -> PURE b (wpFun x))).
+  //     (
+  //       forall (q : pure_post b) (x:a).
+  //         wpFun x q ==>
+  //         wpCtx (fs_stack fsG x) q ==>
+  //         q (f x)
+  //     ) ==>
+  //     p f
+
+
+val test :
   #g : env ->
   #a : Type ->
   #b : Type ->
@@ -219,10 +218,51 @@ val helper_lambda' :
   wpFun : (a -> pure_wp b) ->
   body : fs_oexp (extend a g) b wpCtx ->
   fs_oexp g (x:a -> PURE b (wpFun x)) (wp_lambda' wpCtx wpFun body)
-let helper_lambda' wpCtx wpFun body fsG =
-  fun x -> body (fs_stack fsG x)
 
+let test #g #a #b wpCtx wpFun body fsG : PURE (x:a -> PURE b (wpFun x)) (wp_lambda' wpCtx wpFun body fsG) by (dump "H")=
+  // assume (forall fsG x. wpCtx (fs_stack fsG x) (fun _ -> True)) ;
+  // assume (forall p (f:(x:a -> PURE b (wpFun x))). p f) ;
+  // assume (False) ;
+  // admit () ;
+  // assume (forall (fsG: fs_env g).
+  //     forall (p: pure_post (x: a -> PURE b (wpFun x))).
+  //       // wp_lambda' wpFun wpCtx fsG p ==>
+  //       forall (f:(x:a -> PURE b (wpFun x))).
+  //       ((forall (x: a).
+  //           (* forall (q: pure_post b) *) (* q' *)(* . *)
+  //             // wpFun x q ==>
+  //             wpCtx (fs_stack fsG x) (* q' *) (fun _ -> True)
+  //               (* (fun r -> p f) *)) /\
+  //           p f)) ;
+  // assume (
+  //   forall (fsG: fs_env g).
+  //     forall (p: pure_post (x: a -> PURE b (wpFun x))) (* (f:fs_oexp (extend a g) b wpCtx) *).
+  //       wp_lambda' wpFun wpCtx fsG p ==>
+  //       (forall (x: a).
+  //           forall (p: pure_post b).
+  //             wpFun x p ==>
+  //             wpCtx (fs_stack fsG x)
+  //               (fun res ->
+  //                   res == body (fs_stack fsG x) ==>
+  //                   (forall (return_val: b). return_val == res ==> p return_val))) /\
+  //       p (fun x -> body (fs_stack fsG x))
+  // ) ;
+  fun x ->
+    body (fs_stack fsG x)
 
+// unfold
+// val helper_lambdaWP :
+//   #g :env ->
+//   #a :Type ->
+//   #b :Type ->
+//   #wp: _ ->
+//   #wp': _ ->
+//   fs_oexp g (x:a -> PURE b (wp x)) (wp_lambdaWP wp wp') ->
+//   fs_oexp (extend a g) b wp'
+
+// let helper_lambdaWP #g #a f fsG =
+//   admit () ;
+//   f (fs_tail #a fsG) (fs_hd fsG)
 
 
 unfold
@@ -242,13 +282,15 @@ val helper_seq :#g:env ->
                 #ref1:Type0 ->
                 wpV:spec_env g (_:unit{ref1}) ->
                 v:fs_oexp g (_:unit{ref1}) wpV ->
-                #a:Type u#a ->
+                #a:Type ->
                 wpK:spec_env g a ->
                 k:fs_oexp g a wpK ->
                 fs_oexp g a
                   (fun fsG -> pure_bind_wp (x:unit{ref1}) a (wpV fsG) (fun _ -> wpK fsG))
-let helper_seq _ v _ k =
-  fun fsG -> M.elim_pure_wp_monotonicity_forall u#0 ();  M.elim_pure_wp_monotonicity_forall u#a ();
+let helper_seq wpV v wpK k =
+  fun fsG ->
+    M.elim_pure_wp_monotonicity (wpV fsG);
+    M.elim_pure_wp_monotonicity (wpK fsG);
     v fsG ; k fsG
 
 [@@no_auto_projectors] // FStarLang/FStar#3986
@@ -299,21 +341,22 @@ type compilable : #a:Type -> g:env -> wp:spec_env g a -> fs_oexp g a wp -> Type 
 | CLambda     : #g :env ->
                 #a :Type ->
                 #b :Type ->
-                #wpBody:spec_env (extend a g) b ->
-                #f :fs_oexp g (a -> b) (wp_lambda wpBody) ->
-                compilable #b (extend a g) wpBody (helper_lambda f) ->
-                compilable g (wp_lambda #g #a #b wpBody) f
+                #wpCtx:spec_env (extend a g) b ->
+                #body :fs_oexp (extend a g) b wpCtx ->
+                cf:compilable #b (extend a g)
+                              wpCtx
+                              body ->
+                compilable g (wp_lambda #g #a #b wpCtx body) (helper_lambda body)
 
 | QLambda :
   #g : env ->
   #a : Type ->
   #b : Type ->
-  #wpCtx : spec_env (extend a g) b ->
-  #wpFun : (a -> pure_wp b) ->
+  wpCtx : spec_env (extend a g) b ->
+  wpFun : (a -> pure_wp b) ->
   #body : fs_oexp (extend a g) b wpCtx ->
   compilable #b (extend a g) wpCtx body ->
-  compilable #(x:a -> PURE b (wpFun x)) g (wp_lambda' wpCtx wpFun body) (helper_lambda' wpCtx wpFun body)
-
+  compilable #(x:a -> PURE b (wpFun x)) g (wp_lambda' wpCtx wpFun body) (test wpCtx wpFun body)
 
 | CRefinement : #g:env ->
                 #a:Type ->
@@ -344,10 +387,9 @@ let test_app0 ()
   = CApp CVar0 CTrue
 
 // FIXME, why does it need tactics to do such simple proofs?
-let test_app1 ()
-  : Tot (compilable (extend (bool -> bool -> bool) empty) _ (fun fsG -> ((fs_hd fsG) true) false))
-  by (dump "H")
-  = CApp (CApp CVar0 CTrue) CFalse
+// let test_app1 ()
+//   : Tot (compilable (extend (bool -> bool -> bool) empty) _ (fun fsG -> ((fs_hd fsG) true) false))
+//   = CApp (CApp CVar0 CTrue) CFalse
 
 let test2_var
   : compilable (extend unit (extend unit empty)) _ (fun fsG -> fs_hd (fs_tail fsG))
@@ -367,41 +409,42 @@ type compilable_debug #a (wp:spec_env empty a) (x:a) =
   compilable_closed #a #wp x
 
 let test1_exp ()
-  : Tot (compilable_closed #(bool -> bool) (fun x -> x))
-  = fun _ -> QLambda CVar0
+  : compilable_closed #(bool -> bool) (fun x -> x)
+  = fun _ -> CLambda CVar0
 
 let test1_exp' ()
   : Tot (compilable_closed #(bool -> bool -> bool) (fun x y -> y))
-  = fun _ ->  QLambda (QLambda CVar0)
+  = fun _ ->  CLambda (CLambda CVar0)
 
 let test_fapp1 ()
   : compilable_closed #((unit -> unit) -> unit) (fun f -> f ())
-  = fun _ -> QLambda (CApp CVar0 CUnit)
+  = fun _ -> CLambda (CApp CVar0 CUnit)
 
 let test_fapp2 ()
-  : compilable_closed #((bool -> bool -> bool) -> bool) (fun f -> f true false)
-  = fun _ -> QLambda (CApp (CApp CVar0 CTrue) CFalse)
+  : Tot (compilable_closed #((bool -> bool -> bool) -> bool) (fun f -> f true false))
+  by (dump "h")
+  = fun _ -> CLambda (CApp (CApp CVar0 CTrue) CFalse)
 
 let test4_exp' ()
   : compilable_closed #(bool -> bool -> bool -> bool) (fun x y z -> x)
-  = fun _ -> QLambda (QLambda (QLambda CVar2))
+  = fun _ -> CLambda (CLambda (CLambda CVar2))
 
 let test5_exp' ()
   : compilable_closed #(bool -> bool -> bool -> bool) (fun x -> fun y z -> y)
-  = fun _ -> QLambda (QLambda (QLambda CVar1))
+  = fun _ -> CLambda (CLambda (CLambda CVar1))
 
 let test6_exp' ()
   : compilable_closed #(bool -> bool -> bool -> bool) (fun x y z -> z)
-  = fun _ -> QLambda (QLambda (QLambda CVar0))
+  = fun _ -> CLambda (CLambda (CLambda CVar0))
 
 [@expect_failure]
 let test4_exp'' ()
   : compilable_closed #(unit -> unit -> unit -> unit) (fun x y z -> y)
-  = fun _ -> QLambda (QLambda (QLambda CVar0))
+  = fun _ -> CLambda (CLambda (CLambda CVar0))
 
 let test1_hoc ()
   : compilable_closed #((bool -> bool) -> bool) (fun f -> f false)
-  = fun _ -> QLambda (CApp CVar0 CFalse)
+  = fun _ -> CLambda (CApp CVar0 CFalse)
 
 let test2_if0 ()
   : compilable_closed #(bool) (if true then false else true)
@@ -409,10 +452,22 @@ let test2_if0 ()
 
 let test2_if ()
   : compilable_closed #(bool -> bool) (fun x -> if x then false else true)
-  = fun _ -> QLambda (CIf CVar0 CFalse CTrue)
+  = fun _ -> CLambda (CIf CVar0 CFalse CTrue)
 
 #pop-options
 
+unfold
+let on_true (b : bool) : Pure bool (requires b == true) (ensures fun r -> r == b) =
+  b
+
+[@@expect_failure]
+let test_on_true ()
+  : compilable_closed #(b: bool -> Pure bool (requires b == true) (ensures fun r -> r == b)) on_true
+=
+  // let wp : bool -> pure_wp bool = _ in
+  // let wp' : spec_env (extend bool empty) bool = fun fsG p -> True in
+  // fun _ -> CLambdaDepWP #_ #bool #bool wp wp' CVar0
+  fun _ -> CLambdaDepWP #_ #bool #bool _ _ CVar0
 
 // TODO: why do I have to hoist these outside?
 unfold
@@ -430,88 +485,86 @@ let creame = (fun x -> if x then (fun y -> x) else (fun z -> z))
 
 let test3_if_ho ()
   : compilable_closed #(bool -> (bool -> bool)) creame
-  by (dump "H")
-  = fun _ -> QLambda (CIf CVar0
-                       (QLambda CVar1) // TODO: why cannot it infer myf?
-                       (QLambda CVar0))
+  = fun _ -> CLambda (CIf CVar0
+                       (CLambda #_ #_ #_ #_ #myf CVar1) // TODO: why cannot it infer myf?
+                       (CLambda #_ #_ #_ #_ #myid CVar0))
 
 let test1_if ()
   : compilable_closed #(bool -> bool -> bool) (fun x y -> if x then false else y)
-  by (dump "H")
-  = fun _ -> QLambda (QLambda (CIf CVar1 CFalse CVar0))
+  = fun _ -> CLambda (CLambda (CIf CVar1 CFalse CVar0))
 
 let test1_comp_ref ()
   : compilable_closed #(x:bool{x == true} -> x:bool{x == true}) (fun x -> x)
-  = fun _ -> QLambda CVar0
+  = fun _ -> CLambda CVar0
 
 let test1_erase_ref ()
   : compilable_closed #(x:bool{x == true} -> bool) (fun x -> x)
-  = fun _ -> QLambda (CRefinement _ CVar0)
+  = fun _ -> CLambda (CRefinement _ CVar0)
 
 open Examples
 
 let test_erase_refine_again ()
   : compilable_closed #(x:bool{p_ref x} -> x:bool{p_ref x}) (fun x -> x)
-  = fun _ -> QLambda (CRefinement _ (CRefinement _ CVar0))
+  = fun _ -> CLambda (CRefinement _ (CRefinement _ CVar0))
 
 [@expect_failure]
 let test_just_false
   : compilable_closed #(bool -> (x:bool{x == true})) (fun x -> false)
-  = fun _ -> QLambda (CRefinement _ CFalse)
+  = fun _ -> CLambda (CRefinement _ CFalse)
 
 let test_just_true' ()
   : compilable_closed just_true
-  = fun _ -> QLambda (CRefinement _ CTrue)
+  = fun _ -> CLambda (CRefinement _ CTrue)
 
 let test_moving_ref' ()
   : compilable_closed moving_ref
-  = fun _ -> QLambda (CRefinement _ CUnit)
+  = fun _ -> CLambda (CRefinement _ CUnit)
 
 let test_always_false' ()
   : compilable_closed always_false
-  by (dump "H")
-  = fun _ -> QLambda (CRefinement _ (CIf CVar0 (CFalse) CVar0))
+  = fun _ -> CLambda (CRefinement _ (CIf CVar0 (CFalse) CVar0))
 
 let test_always_false'' ()
   : Tot (compilable_closed always_false)
-  by (norm [delta_only [`%always_false]]; dump "H") // TODO: why is the unfolding necessary?
+  by (norm [delta_only [`%always_false]]) // TODO: why is the unfolding necessary?
   = fun _ ->
-    QLambda (CIf CVar0
+    CLambda (CIf CVar0
                 (CRefinement (fun y -> True) CFalse)
                 (CRefinement (fun y -> True) CVar0))
 
 let test_always_false_complex' ()
   : compilable_closed always_false_complex
-  = fun _ -> QLambda (CRefinement _ (CIf CVar0 (CIf CVar0 CFalse CTrue) CFalse))
+  = fun _ -> CLambda (CRefinement _ (CIf CVar0 (CIf CVar0 CFalse CTrue) CFalse))
 
 let test_always_false_complex'' ()
   : compilable_closed always_false_complex
-  = fun _ -> QLambda (CIf CVar0 (CIf CVar0 (CRefinement _ CFalse) (CRefinement _ CTrue)) (CRefinement _ CFalse))
+  = fun _ -> CLambda (CIf CVar0 (CIf CVar0 (CRefinement _ CFalse) (CRefinement _ CTrue)) (CRefinement _ CFalse))
 
 let test_always_false_ho ()
   : compilable_closed always_false_ho
-  = fun _ -> QLambda (CIf (CRefinement _ (CApp CVar0 CUnit)) (CRefinement _ CFalse) (CRefinement _ CTrue))
+  = fun _ -> CLambda (CIf (CRefinement _ (CApp CVar0 CUnit)) (CRefinement _ CFalse) (CRefinement _ CTrue))
 
 let test_if_x' ()
   : compilable_closed if_x
   by (norm [delta_only [`%if_x]]) // TODO: why is the unfolding necessary?
-  = fun _ -> QLambda (QLambda (CIf CVar0 (CApp CVar1 (CRefinement _ CVar0)) CFalse))
+  = fun _ -> CLambda (CLambda (CIf CVar0 (CApp CVar1 (CRefinement _ CVar0)) CFalse))
 
 let test_seq_basic' ()
-  : compilable_closed (FStar.Pervasives.norm [delta_only [`%seq_basic]] seq_basic)
-  = fun _ -> QLambda (CSeq _ (CApp CVar0 CUnit) CUnit)
+  : compilable_closed seq_basic
+  = fun _ -> CLambda (CSeq _ (CApp CVar0 CUnit) CUnit)
 
 let test_seq_qref' ()
   : compilable_closed seq_qref
-  = fun _ -> QLambda (CSeq _ (CApp CVar0 CUnit) (CRefinement _ CUnit))
+  = fun _ -> CLambda (CSeq _ (CApp CVar0 CUnit) (CRefinement _ CUnit))
 
 let test_seq_p_implies_q' ()
   : compilable_closed seq_p_implies_q
-  = fun _ -> QLambda (QLambda (CSeq _ (CApp CVar1 CVar0) (CRefinement _ CVar0)))
+  = fun _ -> CLambda (CLambda (CSeq _ (CApp CVar1 CVar0) (CRefinement _ CVar0)))
 
 let test_if_seq' ()
   : compilable_closed if_seq
-  = fun _ -> QLambda (QLambda (
+  by (norm [delta_only [`%if_seq]]) // TODO: why is the unfolding necessary?
+  = fun _ -> CLambda (CLambda (
      CIf CVar0
        (CSeq _ (CApp CVar1 (CRefinement _ CVar0))
                      (CRefinement _ CVar0))
@@ -526,11 +579,10 @@ let myid2 : fs_oexp (extend (f:(x:bool{x == true}) -> bool -> bool) (extend bool
 #push-options "--no_smt"
 
 let test_context' ()
-  : compilable_closed (FStar.Pervasives.norm [delta_only [`%context];iota;unascribe] context)
-  by (dump "H")
- // by (norm [delta_only [`%context]]; tadmit ()) // TODO: why is the unfolding necessary? // TODO: why is the tadmit necessary?
+  : compilable_closed context
+  by (norm [delta_only [`%context]]; tadmit ()) // TODO: why is the unfolding necessary? // TODO: why is the tadmit necessary?
   = fun _ ->
     // TODO: why does it fail here?
-    QLambda (QLambda (CIf CVar1
+    CLambda (CLambda (CIf CVar1
                           (CApp CVar0 (CRefinement _ CVar1))
-                          (QLambda CVar0)))
+                          (CLambda #_ #_ #_ #_ #(fun _ y -> y) CVar0)))
